progress and preservation for arith

arith.lean
@@ -6,19 +6,6 @@ inductive typ : Type
   | num : typ
   | bool : typ
 
-lemma typ_cases {p: Prop} (t: typ)
-    (num_case: t = typ.num → p)
-    (bool_case: t = typ.bool → p): p :=
-  begin
-    induction t,
-    case typ.num {
-      apply num_case rfl
-    },
-    case typ.bool {
-      apply bool_case rfl
-    }
-  end
-
 inductive exp : Type
   | num : ℕ → exp
   | bool : bool → exp
@@ -30,22 +17,9 @@ inductive is_value : exp → Prop
   | num {n: ℕ} : is_value (exp.num n)
   | bool {b: bool} : is_value (exp.bool b)
 
-lemma is_value_cases {p: Prop} {e: exp} (e_is_value: is_value e)
-    (num_case: ∀ (n: ℕ), e = exp.num n → p)
-    (bool_case: ∀ (b: bool), e = exp.bool b → p): p :=
-  begin
-    induction e_is_value,
-    case is_value.num n {
-      apply num_case n rfl
-    },
-    case is_value.bool b {
-      apply bool_case b rfl
-    }
-  end
-
 inductive step : exp → exp → Prop
   notation e1 `⟶` e2:100 := step e1 e2
-  | add {n1 n2: ℕ}:             exp.add (exp.num n1) (exp.num n2) ⟶ exp.num (n1 +n2)
+  | add {n1 n2: ℕ}:             exp.add (exp.num n1) (exp.num n2) ⟶ exp.num (n1+n2)
   | add_right {e1 e2 e2': exp}: is_value e1 → (e2 ⟶ e2') →
                                 (exp.add e1 e2 ⟶ exp.add e1 e2')
   | add_left {e1 e1' e2: exp}:  (e1 ⟶ e1') →
@@ -63,6 +37,13 @@ inductive step : exp → exp → Prop
 
 notation e1 `⟶` e2:100 := step e1 e2
 
+inductive trans_step : exp → exp → Prop
+  notation e `⟶*` e':100 := trans_step e e'
+  | rfl {e: exp}:          e ⟶* e
+  | trans {e e' e'': exp}: (e ⟶ e') → (e' ⟶* e'') → (e ⟶* e'')
+
+notation e `⟶*` e':100 := trans_step e e'
+
 inductive typed : exp → typ → Prop
   notation e1 `:::` e2:100 := typed e1 e2
   | num {n: ℕ}:                   exp.num n ::: typ.num
@@ -75,6 +56,80 @@ inductive typed : exp → typ → Prop
                                   (exp.eq e1 e2 ::: typ.bool)
 
 notation e1 `:::` e2:100 := typed e1 e2
+
+lemma of_not_not{α: Prop} (p: ¬ ¬ α) : α :=
+  or.elim (classical.em α) id (flip absurd p)
+
+lemma typ_cases {p: Prop} (t: typ)
+    (num_case: t = typ.num → p)
+    (bool_case: t = typ.bool → p): p :=
+  begin
+    induction t,
+    case typ.num {
+      apply num_case rfl
+    },
+    case typ.bool {
+      apply bool_case rfl
+    }
+  end
+
+lemma is_value_cases {p: Prop} {e: exp} (e_is_value: is_value e)
+    (num_case: ∀ (n: ℕ), e = exp.num n → p)
+    (bool_case: ∀ (b: bool), e = exp.bool b → p): p :=
+  begin
+    induction e_is_value,
+    case is_value.num n {
+      apply num_case n rfl
+    },
+    case is_value.bool b {
+      apply bool_case b rfl
+    }
+  end
+
+lemma step_cases {p: Prop} {e e': exp} (e_steps: e ⟶ e')
+    (add_case: ∀ (n1 n2: ℕ), e = exp.add (exp.num n1) (exp.num n2) → e' = exp.num (n1+n2) → p)
+    (add_right_case: ∀ (e1 e2 e2': exp), is_value e1 → (e2 ⟶ e2') → e = exp.add e1 e2 → e' = exp.add e1 e2' → p)
+    (add_left_case: ∀ (e1 e1' e2: exp), (e1 ⟶ e1') → e = exp.add e1 e2 → e' = exp.add e1' e2 → p)
+    (ite_true_case: ∀ (e2 e3: exp), e = exp.ite (exp.bool true) e2 e3 → e' = e2 → p)
+    (ite_false_case: ∀ (e2 e3: exp), e = exp.ite (exp.bool false) e2 e3 → e' = e3 → p)
+    (ite_case: ∀ (e1 e1' e2 e3: exp), e1 ⟶ e1' → e = exp.ite e1 e2 e3 → e' = exp.ite e1' e2 e3 → p)
+    (eq_num_case: ∀ (n1 n2: ℕ), e = exp.eq (exp.num n1) (exp.num n2) → e' = exp.bool (n1 = n2) → p)
+    (eq_bool_case: ∀ (b1 b2: bool), e = exp.eq (exp.bool b1) (exp.bool b2) → e' = exp.bool (b1 = b2) → p)
+    (eq_right_case: ∀ (e1 e2 e2': exp), is_value e1 → (e2 ⟶ e2') → e = exp.eq e1 e2 → e' = exp.eq e1 e2' → p)
+    (eq_left_case: ∀ (e1 e1' e2: exp), (e1 ⟶ e1') → e = exp.eq e1 e2 → e' = exp.eq e1' e2 → p) : p :=
+  begin
+    induction e_steps,
+    case step.add n1 n2 {
+      apply add_case n1 n2 rfl rfl
+    },
+    case step.add_right e1 e2 e2' e1_is_value e2_steps {
+      apply add_right_case e1 e2 e2' e1_is_value e2_steps rfl rfl
+    },
+    case step.add_left e1 e1' e2 e1_steps {
+      apply add_left_case e1 e1' e2 e1_steps rfl rfl
+    },
+    case step.ite_true e2 e3 {
+      apply ite_true_case e2 e3 rfl rfl
+    },
+    case step.ite_false e2 e3 {
+      apply ite_false_case e2 e3 rfl rfl
+    },
+    case step.ite e1 e1' e2 e3 e1_steps {
+      apply ite_case e1 e1' e2 e3 e1_steps rfl rfl
+    },
+    case step.eq_num n1 n2 {
+      apply eq_num_case n1 n2 rfl rfl
+    },
+    case step.eq_bool b1 b2 {
+      apply eq_bool_case b1 b2 rfl rfl
+    },
+    case step.eq_right e1 e2 e2' e1_is_value e2_steps {
+      apply eq_right_case e1 e2 e2' e1_is_value e2_steps rfl rfl
+    },
+    case step.eq_left e1 e1' e2 e1_steps {
+      apply eq_left_case e1 e1' e2 e1_steps rfl rfl
+    }
+  end
 
 lemma typed_cases {p: Prop} {e: exp} {t: typ} (e_typed_t: e ::: t)
     (num_case: ∀ (n: ℕ), e = exp.num n → t = typ.num → p)
@@ -101,7 +156,55 @@ lemma typed_cases {p: Prop} {e: exp} {t: typ} (e_typed_t: e ::: t)
     },
   end
 
-lemma numt_inversion {e: exp} (e_typed_num: e ::: typ.num) (e_is_val: is_value e): ∃n: ℕ, e = exp.num n :=
+lemma add_is_not_value {e1 e2: exp} : ¬ is_value (exp.add e1 e2) :=
+  classical.by_contradiction (
+    assume add_is_value: ¬¬ is_value (exp.add e1 e2),
+    is_value_cases (of_not_not add_is_value)
+    (  -- is value num
+      assume n: ℕ,
+      assume add_is_num: exp.add e1 e2 = exp.num n,
+      show false, from exp.no_confusion add_is_num
+    )
+    (  -- is value bool
+      assume b: bool,
+      assume add_is_bool: exp.add e1 e2 = exp.bool b,
+      show false, from exp.no_confusion add_is_bool
+    )
+  )
+
+lemma ite_is_not_value {e1 e2 e3: exp} : ¬ is_value (exp.ite e1 e2 e3) :=
+  classical.by_contradiction (
+    assume ite_is_value: ¬¬ is_value (exp.ite e1 e2 e3),
+    is_value_cases (of_not_not ite_is_value)
+    (  -- is value num
+      assume n: ℕ,
+      assume add_is_num: exp.ite e1 e2 e3 = exp.num n,
+      show false, from exp.no_confusion add_is_num
+    )
+    (  -- is value bool
+      assume b: bool,
+      assume add_is_bool: exp.ite e1 e2 e3 = exp.bool b,
+      show false, from exp.no_confusion add_is_bool
+    )
+  )
+
+lemma eq_is_not_value {e1 e2: exp} : ¬ is_value (exp.eq e1 e2) :=
+  classical.by_contradiction (
+    assume eq_is_value: ¬¬ is_value (exp.eq e1 e2),
+    is_value_cases (of_not_not eq_is_value)
+    (  -- is value num
+      assume n: ℕ,
+      assume add_is_num: exp.eq e1 e2 = exp.num n,
+      show false, from exp.no_confusion add_is_num
+    )
+    (  -- is value bool
+      assume b: bool,
+      assume add_is_bool: exp.eq e1 e2 = exp.bool b,
+      show false, from exp.no_confusion add_is_bool
+    )
+  )
+
+lemma value_typed_num_is_num {e: exp} (e_typed_num: e ::: typ.num) (e_is_value: is_value e): ∃n: ℕ, e = exp.num n :=
   typed_cases e_typed_num
   ( -- num
     assume n: ℕ,
@@ -119,59 +222,26 @@ lemma numt_inversion {e: exp} (e_typed_num: e ::: typ.num) (e_is_val: is_value e
     assume _ _,
     assume e_is_add: e = exp.add e1 e2,
     assume _,
-    is_value_cases e_is_val
-    (  -- is value num
-      assume n: ℕ,
-      assume e_is_num: e = exp.num n,
-      have add_is_num: exp.add e1 e2 = exp.num n, from eq.trans (eq.symm e_is_add) e_is_num,
-      show ∃n: ℕ, e = exp.num n, from exp.no_confusion add_is_num
-    )
-    (  -- is value bool
-      assume b: bool,
-      assume e_is_bool: e = exp.bool b,
-      have add_is_bool: exp.add e1 e2 = exp.bool b, from eq.trans (eq.symm e_is_add) e_is_bool,
-      show ∃n: ℕ, e = exp.num n, from exp.no_confusion add_is_bool
-    )
+    have add_is_value: is_value (exp.add e1 e2), by { rw[e_is_add] at e_is_value, assumption },
+    show ∃n: ℕ, e = exp.num n, from absurd add_is_value add_is_not_value
   )
   ( -- ite
     assume e1 e2 e3: exp,
     assume _ _ _,
     assume e_is_ite: e = exp.ite e1 e2 e3,
-    is_value_cases e_is_val
-    (  -- is value num
-      assume n: ℕ,
-      assume e_is_num: e = exp.num n,
-      have add_is_num: exp.ite e1 e2 e3 = exp.num n, from eq.trans (eq.symm e_is_ite) e_is_num,
-      show ∃n: ℕ, e = exp.num n, from exp.no_confusion add_is_num
-    )
-    (  -- is value bool
-      assume b: bool,
-      assume e_is_bool: e = exp.bool b,
-      have add_is_bool: exp.ite e1 e2 e3 = exp.bool b, from eq.trans (eq.symm e_is_ite) e_is_bool,
-      show ∃n: ℕ, e = exp.num n, from exp.no_confusion add_is_bool
-    )
+    have ite_is_value: is_value (exp.ite e1 e2 e3), by { rw[e_is_ite] at e_is_value, assumption },
+    show ∃n: ℕ, e = exp.num n, from absurd ite_is_value ite_is_not_value
   )
   ( -- eq
     assume e1 e2: exp,
     assume _ _ _,
     assume e_is_eq: e = exp.eq e1 e2,
     assume _,
-    is_value_cases e_is_val
-    (  -- is value num
-      assume n: ℕ,
-      assume e_is_num: e = exp.num n,
-      have add_is_num: exp.eq e1 e2 = exp.num n, from eq.trans (eq.symm e_is_eq) e_is_num,
-      show ∃n: ℕ, e = exp.num n, from exp.no_confusion add_is_num
-    )
-    (  -- is value bool
-      assume b: bool,
-      assume e_is_bool: e = exp.bool b,
-      have add_is_bool: exp.eq e1 e2 = exp.bool b, from eq.trans (eq.symm e_is_eq) e_is_bool,
-      show ∃n: ℕ, e = exp.num n, from exp.no_confusion add_is_bool
-    )
+    have eq_is_value: is_value (exp.eq e1 e2), by { rw[e_is_eq] at e_is_value, assumption },
+    show ∃n: ℕ, e = exp.num n, from absurd eq_is_value eq_is_not_value
   )
 
-lemma boolt_inversion {e: exp} (e_typed_bool: e ::: typ.bool) (e_is_val: is_value e):
+lemma value_typed_bool_is_true_or_false {e: exp} (e_typed_bool: e ::: typ.bool) (e_is_value: is_value e):
                       e = exp.bool true ∨ e = exp.bool false :=
   typed_cases e_typed_bool
   ( -- num
@@ -200,260 +270,734 @@ lemma boolt_inversion {e: exp} (e_typed_bool: e ::: typ.bool) (e_is_val: is_valu
     assume _ _,
     assume e_is_add: e = exp.add e1 e2,
     assume _,
-    is_value_cases e_is_val
-    (  -- is value num
-      assume n: ℕ,
-      assume e_is_num: e = exp.num n,
-      have add_is_num: exp.add e1 e2 = exp.num n, from eq.trans (eq.symm e_is_add) e_is_num,
-      show e = exp.bool true ∨ e = exp.bool false, from exp.no_confusion add_is_num
-    )
-    (  -- is value bool
-      assume b: bool,
-      assume e_is_bool: e = exp.bool b,
-      have add_is_bool: exp.add e1 e2 = exp.bool b, from eq.trans (eq.symm e_is_add) e_is_bool,
-      show e = exp.bool true ∨ e = exp.bool false, from exp.no_confusion add_is_bool
-    )
+    have add_is_value: is_value (exp.add e1 e2), by { rw[e_is_add] at e_is_value, assumption },
+    show e = exp.bool true ∨ e = exp.bool false, from absurd add_is_value add_is_not_value
   )
   ( -- ite
     assume e1 e2 e3: exp,
     assume _ _ _,
     assume e_is_ite: e = exp.ite e1 e2 e3,
-    is_value_cases e_is_val
-    (  -- is value num
-      assume n: ℕ,
-      assume e_is_num: e = exp.num n,
-      have add_is_num: exp.ite e1 e2 e3 = exp.num n, from eq.trans (eq.symm e_is_ite) e_is_num,
-      show e = exp.bool true ∨ e = exp.bool false, from exp.no_confusion add_is_num
-    )
-    (  -- is value bool
-      assume b: bool,
-      assume e_is_bool: e = exp.bool b,
-      have add_is_bool: exp.ite e1 e2 e3 = exp.bool b, from eq.trans (eq.symm e_is_ite) e_is_bool,
-      show e = exp.bool true ∨ e = exp.bool false, from exp.no_confusion add_is_bool
-    )
+    have ite_is_value: is_value (exp.ite e1 e2 e3), by { rw[e_is_ite] at e_is_value, assumption },
+    show e = exp.bool true ∨ e = exp.bool false, from absurd ite_is_value ite_is_not_value
   )
   ( -- eq
     assume e1 e2: exp,
     assume _ _ _,
     assume e_is_eq: e = exp.eq e1 e2,
     assume _,
-    is_value_cases e_is_val
-    (  -- is value num
-      assume n: ℕ,
-      assume e_is_num: e = exp.num n,
-      have add_is_num: exp.eq e1 e2 = exp.num n, from eq.trans (eq.symm e_is_eq) e_is_num,
-      show e = exp.bool true ∨ e = exp.bool false, from exp.no_confusion add_is_num
-    )
-    (  -- is value bool
-      assume b: bool,
-      assume e_is_bool: e = exp.bool b,
-      have add_is_bool: exp.eq e1 e2 = exp.bool b, from eq.trans (eq.symm e_is_eq) e_is_bool,
-      show e = exp.bool true ∨ e = exp.bool false, from exp.no_confusion add_is_bool
-    )
+    have eq_is_value: is_value (exp.eq e1 e2), by { rw[e_is_eq] at e_is_value, assumption },
+    show e = exp.bool true ∨ e = exp.bool false, from absurd eq_is_value eq_is_not_value
   )
 
-theorem progress(e: exp) (t: typ) (is_typed: e ::: t): is_value e ∨ ∃e', e ⟶ e' :=
-  typed.rec_on is_typed
-    ( -- num
-      assume n: ℕ,
-      let e := exp.num n in
-      have e_is_val: is_value e, from is_value.num,
-      show is_value e ∨ ∃e', e ⟶ e', from or.inl e_is_val
+lemma bool_eq_bool_steps {e: exp} {b1 b2: bool} (e_is_eq: e = exp.eq (exp.bool b1) (exp.bool b2)):
+  ∃e', e ⟶ e' :=
+  have exp.eq (exp.bool b1) (exp.bool b2) ⟶ exp.bool (b1 = b2), from step.eq_bool,
+  have ∃e', exp.eq (exp.bool b1) (exp.bool b2) ⟶ e', from exists.intro (exp.bool (b1 = b2)) this,
+  show ∃e', e ⟶ e', by { rw [←e_is_eq] at this, assumption }
+
+theorem progress(e: exp) (t: typ) (e_typed_t: e ::: t): is_value e ∨ ∃e', e ⟶ e' :=
+  typed.rec_on e_typed_t
+  ( -- num
+    assume n: ℕ,
+    let e := exp.num n in
+    have e_is_value: is_value e, from is_value.num,
+    show is_value e ∨ ∃e', e ⟶ e', from or.inl e_is_value
+  )
+  ( -- bool
+    assume b: bool,
+    let e := exp.bool b in
+    have e_is_value: is_value e, from is_value.bool,
+    show is_value e ∨ ∃e', e ⟶ e', from or.inl e_is_value
+  )
+  ( -- add
+    assume e1 e2: exp,
+    assume e1_typed_num : e1 ::: typ.num,
+    assume e2_typed_num : e2 ::: typ.num,
+    assume e1ih: is_value e1 ∨ ∃e1', e1 ⟶ e1',
+    assume e2ih: is_value e2 ∨ ∃e2', e2 ⟶ e2',
+    let e := exp.add e1 e2 in
+    have e_is_add: e = exp.add e1 e2, from rfl,
+    have e_steps: ∃e', e ⟶ e', from or.elim e1ih (
+      assume e1_is_value: is_value e1,
+      or.elim e2ih (
+        assume e2_is_value: is_value e2,
+        have e1_exists_num: ∃n1: ℕ, e1 = exp.num n1, from value_typed_num_is_num e1_typed_num e1_is_value,
+        have e2_exists_num: ∃n2: ℕ, e2 = exp.num n2, from value_typed_num_is_num e2_typed_num e2_is_value,
+        exists.elim e1_exists_num (
+          assume n1: ℕ,
+          assume e1_is_num: e1 = exp.num n1,
+          exists.elim e2_exists_num (
+            assume n2: ℕ,
+            assume e2_is_num: e2 = exp.num n2,
+            have exp.add (exp.num n1) (exp.num n2) ⟶ exp.num (n1 + n2), from step.add,
+            have e ⟶ exp.num (n1 + n2), by { rw [←e1_is_num, ←e2_is_num, ←e_is_add] at this, assumption },
+            show ∃e', e ⟶ e', from exists.intro (exp.num (n1 + n2)) this
+          )
+        )
+      )
+      (
+        assume e2_can_step: ∃e2', e2 ⟶ e2',
+        exists.elim e2_can_step (
+          assume e2': exp,
+          assume e2_steps: e2 ⟶ e2',
+          have e ⟶ exp.add e1 e2', from step.add_right e1_is_value e2_steps,
+          show ∃e', e ⟶ e', from exists.intro (exp.add e1 e2') this
+        )
+      )
     )
-    ( -- bool
-      assume b: bool,
-      let e := exp.bool b in
-      have e_is_val: is_value e, from is_value.bool,
-      show is_value e ∨ ∃e', e ⟶ e', from or.inl e_is_val
+    (
+      assume e1_can_step: ∃e1', e1 ⟶ e1',
+      exists.elim e1_can_step (
+        assume e1': exp,
+        assume e1_steps: e1 ⟶ e1',
+        have e ⟶ exp.add e1' e2, from step.add_left e1_steps,
+        show ∃e', e ⟶ e', from exists.intro (exp.add e1' e2) this
+      )
+    ),
+    show is_value e ∨ ∃e', e ⟶ e', from or.inr e_steps
+  )
+  ( -- ite
+    assume e1 e2 e3: exp,
+    assume t: typ,
+    assume e1_typed_bool: e1 ::: typ.bool,
+    assume e2_typed_t: e2 ::: t,
+    assume e3_typed_t: e3 ::: t,
+    assume e1ih: is_value e1 ∨ ∃e1', e1 ⟶ e1',
+    assume e2ih: is_value e2 ∨ ∃e2', e2 ⟶ e2',
+    assume e3ih: is_value e3 ∨ ∃e3', e3 ⟶ e3',
+    let e := exp.ite e1 e2 e3 in
+    have e_is_ite: e = exp.ite e1 e2 e3, from rfl,
+    have e_steps: ∃e', e ⟶ e', from or.elim e1ih
+    ( -- is_value e1
+      assume e1_is_value: is_value e1,
+      have e1_is_bool: e1 = exp.bool true ∨ e1 = exp.bool false,
+      from value_typed_bool_is_true_or_false e1_typed_bool e1_is_value,
+      or.elim e1_is_bool
+      ( -- ite-true
+        assume e1_is_true: e1 = exp.bool true,
+        have exp.ite (exp.bool true) e2 e3 ⟶ e2, from step.ite_true,
+        have e ⟶ e2, by { rw [←e1_is_true, ←e_is_ite] at this, assumption },
+        show ∃e', e ⟶ e', from exists.intro e2 this
+      )
+      ( -- ite-false
+        assume e1_is_false: e1 = exp.bool false,
+        have exp.ite (exp.bool false) e2 e3 ⟶ e3, from step.ite_false,
+        have e ⟶ e3, by { rw [←e1_is_false, ←e_is_ite] at this, assumption },
+        show ∃e', e ⟶ e', from exists.intro e3 this
+      )
     )
-    ( -- add
-      assume e1 e2: exp,
-      assume e1_is_numt : e1 ::: typ.num,
-      assume e2_is_numt : e2 ::: typ.num,
-      assume e1ih: is_value e1 ∨ ∃e1', e1 ⟶ e1',
-      assume e2ih: is_value e2 ∨ ∃e2', e2 ⟶ e2',
-      let e := exp.add e1 e2 in
-      have e_is_add: e = exp.add e1 e2, from rfl,
-      have e_steps: ∃e', e ⟶ e', from or.elim e1ih (
-        assume e1_is_val: is_value e1,
-        or.elim e2ih (
-          assume e2_is_val: is_value e2,
-          have e1_exists_num: ∃n1: ℕ, e1 = exp.num n1, from numt_inversion e1_is_numt e1_is_val,
-          have e2_exists_num: ∃n2: ℕ, e2 = exp.num n2, from numt_inversion e2_is_numt e2_is_val,
+    ( -- e1 steps
+      assume e1_can_step: ∃e1', e1 ⟶ e1',
+      exists.elim e1_can_step (
+        assume e1': exp, 
+        assume e1_steps: e1 ⟶ e1',
+        have e ⟶ exp.ite e1' e2 e3, from step.ite e1_steps,
+        show ∃e', e ⟶ e', from exists.intro (exp.ite e1' e2 e3) this
+      )
+    ),
+    show is_value e ∨ ∃e', e ⟶ e', from or.inr e_steps
+  )
+  ( -- eq
+    assume e1 e2: exp,
+    assume t: typ,
+    assume e1_typed_t: e1 ::: t,
+    assume e2_typed_t: e2 ::: t,
+    assume e1ih: is_value e1 ∨ ∃e1', e1 ⟶ e1',
+    assume e2ih: is_value e2 ∨ ∃e2', e2 ⟶ e2',
+    let e := exp.eq e1 e2 in
+    have e_is_eq: e = exp.eq e1 e2, from rfl,
+    have e_steps: ∃e', e ⟶ e', from or.elim e1ih (
+      assume e1_is_value: is_value e1,
+      or.elim e2ih (
+        assume e2_is_value: is_value e2,
+        typ_cases t
+        ( -- num
+          assume t_is_num: t = typ.num,
+          have e1_typed_num: e1 ::: typ.num, by { rw[t_is_num] at e1_typed_t, assumption  },
+          have e2_typed_num: e2 ::: typ.num, by { rw[t_is_num] at e2_typed_t, assumption  },
+          have e1_exists_num: ∃n1: ℕ, e1 = exp.num n1, from value_typed_num_is_num e1_typed_num e1_is_value,
+          have e2_exists_num: ∃n2: ℕ, e2 = exp.num n2, from value_typed_num_is_num e2_typed_num e2_is_value,
           exists.elim e1_exists_num (
             assume n1: ℕ,
             assume e1_is_num: e1 = exp.num n1,
             exists.elim e2_exists_num (
               assume n2: ℕ,
               assume e2_is_num: e2 = exp.num n2,
-              have exp.add (exp.num n1) (exp.num n2) ⟶ exp.num (n1 + n2), from step.add,
-              have e ⟶ exp.num (n1 + n2), by { rw [←e1_is_num, ←e2_is_num, ←e_is_add] at this, assumption },
-              show ∃e', e ⟶ e', from exists.intro (exp.num (n1 + n2)) this
+              have exp.eq (exp.num n1) (exp.num n2) ⟶ exp.bool (n1 = n2), from step.eq_num,
+              have e ⟶ exp.bool (n1 = n2), by { rw [←e1_is_num, ←e2_is_num, ←e_is_eq] at this, assumption },
+              show ∃e', e ⟶ e', from exists.intro (exp.bool (n1 = n2)) this
             )
           )
         )
-        (
-          assume e2_can_step: ∃e2', e2 ⟶ e2',
-          exists.elim e2_can_step (
-            assume e2': exp,
-            assume e2_steps: e2 ⟶ e2',
-            have e ⟶ exp.add e1 e2', from step.add_right e1_is_val e2_steps,
-            show ∃e', e ⟶ e', from exists.intro (exp.add e1 e2') this
+        ( -- bool
+          assume t_is_bool: t = typ.bool,
+          have e1_typed_bool: e1 ::: typ.bool, by { rw[t_is_bool] at e1_typed_t, assumption  },
+          have e2_typed_bool: e2 ::: typ.bool, by { rw[t_is_bool] at e2_typed_t, assumption  },
+          have e1_some_bool: e1 = exp.bool true ∨ e1 = exp.bool false,
+          from value_typed_bool_is_true_or_false e1_typed_bool e1_is_value,
+          have e2_some_bool: e2 = exp.bool true ∨ e2 = exp.bool false,
+          from value_typed_bool_is_true_or_false e2_typed_bool e2_is_value,
+          or.elim e1_some_bool
+          (
+            assume e1_is_true: e1 = exp.bool true,
+            or.elim e2_some_bool
+            (
+              assume e2_is_true: e2 = exp.bool true,
+              have e_is_true_eq_true: e = exp.eq (exp.bool true) (exp.bool true),
+              by { rw [e1_is_true, e2_is_true] at e_is_eq, assumption },
+              show ∃e', e ⟶ e', from bool_eq_bool_steps e_is_true_eq_true
+            )
+            (
+              assume e2_is_false: e2 = exp.bool false,
+              have e_is_true_eq_false: e = exp.eq (exp.bool true) (exp.bool false),
+              by { rw [e1_is_true, e2_is_false] at e_is_eq, assumption },
+              show ∃e', e ⟶ e', from bool_eq_bool_steps e_is_true_eq_false
+            )
+          )
+          (
+            assume e1_is_false: e1 = exp.bool false,
+            or.elim e2_some_bool
+            (
+              assume e2_is_true: e2 = exp.bool true,
+              have e_is_false_eq_true: e = exp.eq (exp.bool false) (exp.bool true),
+              by { rw [e1_is_false, e2_is_true] at e_is_eq, assumption },
+              show ∃e', e ⟶ e', from bool_eq_bool_steps e_is_false_eq_true
+            )
+            (
+              assume e2_is_false: e2 = exp.bool false,
+              have e_is_false_eq_false: e = exp.eq (exp.bool false) (exp.bool false),
+              by { rw [e1_is_false, e2_is_false] at e_is_eq, assumption },
+              show ∃e', e ⟶ e', from bool_eq_bool_steps e_is_false_eq_false
+            )
           )
         )
       )
       (
-        assume e1_can_step: ∃e1', e1 ⟶ e1',
-        exists.elim e1_can_step (
-          assume e1': exp,
-          assume e1_steps: e1 ⟶ e1',
-          have e ⟶ exp.add e1' e2, from step.add_left e1_steps,
-          show ∃e', e ⟶ e', from exists.intro (exp.add e1' e2) this
-        )
-      ),
-      show is_value e ∨ ∃e', e ⟶ e', from or.inr e_steps
-    )
-    ( -- ite
-      assume e1 e2 e3: exp,
-      assume t: typ,
-      assume e1_is_bool: e1 ::: typ.bool,
-      assume e2_is_t: e2 ::: t,
-      assume e3_is_t: e3 ::: t,
-      assume e1ih: is_value e1 ∨ ∃e1', e1 ⟶ e1',
-      assume e2ih: is_value e2 ∨ ∃e2', e2 ⟶ e2',
-      assume e3ih: is_value e3 ∨ ∃e3', e3 ⟶ e3',
-      let e := exp.ite e1 e2 e3 in
-      have e_is_ite: e = exp.ite e1 e2 e3, from rfl,
-      or.elim e1ih
-      ( -- is_value e1
-        assume e1_is_val: is_value e1,
-        have e1_bool: e1 = exp.bool true ∨ e1 = exp.bool false, from boolt_inversion e1_is_bool e1_is_val,
-        or.elim e1_bool
-        ( -- ite-true
-          assume e1_is_true: e1 = exp.bool true,
-          have exp.ite (exp.bool true) e2 e3 ⟶ e2, from step.ite_true,
-          have e ⟶ e2, by { rw [←e1_is_true, ←e_is_ite] at this, assumption },
-          have e_steps: ∃e', e ⟶ e', from exists.intro e2 this,
-          show is_value e ∨ ∃e', e ⟶ e', from or.inr e_steps
-        )
-        ( -- ite-false
-          assume e1_is_false: e1 = exp.bool false,
-          have exp.ite (exp.bool false) e2 e3 ⟶ e3, from step.ite_false,
-          have e ⟶ e3, by { rw [←e1_is_false, ←e_is_ite] at this, assumption },
-          have e_steps: ∃e', e ⟶ e', from exists.intro e3 this,
-          show is_value e ∨ ∃e', e ⟶ e', from or.inr e_steps
-        )
-      )
-      ( -- e1 steps
-        assume e1_can_step: ∃e1', e1 ⟶ e1',
-        exists.elim e1_can_step (λe1', 
-          assume e1_steps: e1 ⟶ e1',
-          have e ⟶ exp.ite e1' e2 e3, from step.ite e1_steps,
-          have e_steps: ∃e', e ⟶ e', from exists.intro (exp.ite e1' e2 e3) this,
-          show is_value e ∨ ∃e', e ⟶ e', from or.inr e_steps
+        assume e2_can_step: ∃e2', e2 ⟶ e2',
+        exists.elim e2_can_step (λe2', 
+          assume e2_steps: e2 ⟶ e2',
+          have e ⟶ exp.eq e1 e2', from step.eq_right e1_is_value e2_steps,
+          show ∃e', e ⟶ e', from exists.intro (exp.eq e1 e2') this
         )
       )
     )
-    ( -- eq
-      assume e1 e2: exp,
-      assume t: typ,
-      assume e1_typed_t: e1 ::: t,
-      assume e2_typed_t: e2 ::: t,
-      assume e1ih: is_value e1 ∨ ∃e1', e1 ⟶ e1',
-      assume e2ih: is_value e2 ∨ ∃e2', e2 ⟶ e2',
-      let e := exp.eq e1 e2 in
-      have e_is_eq: e = exp.eq e1 e2, from rfl,
-      or.elim e1ih (
-        assume e1_is_val: is_value e1,
-        or.elim e2ih (
-          assume e2_is_val: is_value e2,
-          typ_cases t
-          ( -- num
-            assume t_is_num: t = typ.num,
-            have e1_typed_num: e1 ::: typ.num, by { rw[t_is_num] at e1_typed_t, assumption  },
-            have e2_typed_num: e2 ::: typ.num, by { rw[t_is_num] at e2_typed_t, assumption  },
-            have e1_exists_num: ∃n1: ℕ, e1 = exp.num n1, from numt_inversion e1_typed_num e1_is_val,
-            have e2_exists_num: ∃n2: ℕ, e2 = exp.num n2, from numt_inversion e2_typed_num e2_is_val,
-            exists.elim e1_exists_num (λn1, exists.elim e2_exists_num (λn2,
-              assume e2_is_num: e2 = exp.num n2,
-              assume e1_is_num: e1 = exp.num n1,
-              have exp.eq (exp.num n1) (exp.num n2) ⟶ exp.bool (n1 = n2), from step.eq_num,
-              have e ⟶ exp.bool (n1 = n2), by { rw [←e1_is_num, ←e2_is_num, ←e_is_eq] at this, assumption },
-              have e_steps: ∃e', e ⟶ e', from exists.intro (exp.bool (n1 = n2)) this,
-              show is_value e ∨ ∃e', e ⟶ e', from or.inr e_steps
-            ))
-          )
-          ( -- bool
-            assume t_is_bool: t = typ.bool,
-            have e1_typed_bool: e1 ::: typ.bool, by { rw[t_is_bool] at e1_typed_t, assumption  },
-            have e2_typed_bool: e2 ::: typ.bool, by { rw[t_is_bool] at e2_typed_t, assumption  },
-            have e1_some_bool: e1 = exp.bool true ∨ e1 = exp.bool false, from boolt_inversion e1_typed_bool e1_is_val,
-            have e2_some_bool: e2 = exp.bool true ∨ e2 = exp.bool false, from boolt_inversion e2_typed_bool e2_is_val,
-            or.elim e1_some_bool
-            (
-              assume e1_is_true: e1 = exp.bool true,
-              or.elim e2_some_bool
-              (
-                assume e2_is_true: e2 = exp.bool true,
-                have e_is_true_eq_true: e = exp.eq (exp.bool true) (exp.bool true),
-                by { rw [e1_is_true, e2_is_true] at e_is_eq, assumption },
-                have exp.eq (exp.bool true) (exp.bool true) ⟶ exp.bool true, from step.eq_bool,
-                have e ⟶ exp.bool true, by { rw [←e_is_true_eq_true] at this, assumption },
-                have e_steps: ∃e', e ⟶ e', from exists.intro (exp.bool true) this,
-                show is_value e ∨ ∃e', e ⟶ e', from or.inr e_steps
-              )
-              (
-                assume e2_is_false: e2 = exp.bool false,
-                have e_is_true_eq_false: e = exp.eq (exp.bool true) (exp.bool false),
-                by { rw [e1_is_true, e2_is_false] at e_is_eq, assumption },
-                have exp.eq (exp.bool true) (exp.bool false) ⟶ exp.bool false, from step.eq_bool,
-                have e ⟶ exp.bool false, by { rw [←e_is_true_eq_false] at this, assumption },
-                have e_steps: ∃e', e ⟶ e', from exists.intro (exp.bool false) this,
-                show is_value e ∨ ∃e', e ⟶ e', from or.inr e_steps
-              )
-            )
-            (
-              assume e1_is_false: e1 = exp.bool false,
-              or.elim e2_some_bool
-              (
-                assume e2_is_true: e2 = exp.bool true,
-                have e_is_false_eq_true: e = exp.eq (exp.bool false) (exp.bool true),
-                by { rw [e1_is_false, e2_is_true] at e_is_eq, assumption },
-                have exp.eq (exp.bool false) (exp.bool true) ⟶ exp.bool false, from step.eq_bool,
-                have e ⟶ exp.bool false, by { rw [←e_is_false_eq_true] at this, assumption },
-                have e_steps: ∃e', e ⟶ e', from exists.intro (exp.bool false) this,
-                show is_value e ∨ ∃e', e ⟶ e', from or.inr e_steps
-              )
-              (
-                assume e2_is_false: e2 = exp.bool false,
-                have e_is_false_eq_false: e = exp.eq (exp.bool false) (exp.bool false),
-                by { rw [e1_is_false, e2_is_false] at e_is_eq, assumption },
-                have exp.eq (exp.bool false) (exp.bool false) ⟶ exp.bool true, from step.eq_bool,
-                have e ⟶ exp.bool true, by { rw [←e_is_false_eq_false] at this, assumption },
-                have e_steps: ∃e', e ⟶ e', from exists.intro (exp.bool true) this,
-                show is_value e ∨ ∃e', e ⟶ e', from or.inr e_steps
-              )
-            )
-          )
-        )
-        (
-          assume e2_can_step: ∃e2', e2 ⟶ e2',
-          exists.elim e2_can_step (λe2', 
-            assume e2_steps: e2 ⟶ e2',
-            have e ⟶ exp.eq e1 e2', from step.eq_right e1_is_val e2_steps,
-            have e_steps: ∃e', e ⟶ e', from exists.intro (exp.eq e1 e2') this,
-            show is_value e ∨ ∃e', e ⟶ e', from or.inr e_steps
-          )
-        )
-      ) (
-        assume e1_can_step: ∃e1', e1 ⟶ e1',
-        exists.elim e1_can_step (λe1', 
-          assume e1_steps: e1 ⟶ e1',
-          have e ⟶ exp.eq e1' e2, from step.eq_left e1_steps,
-          have e_steps: ∃e', e ⟶ e', from exists.intro (exp.eq e1' e2) this,
-          show is_value e ∨ ∃e', e ⟶ e', from or.inr e_steps
-        )
+    (
+      assume e1_can_step: ∃e1', e1 ⟶ e1',
+      exists.elim e1_can_step (λe1', 
+        assume e1_steps: e1 ⟶ e1',
+        have e ⟶ exp.eq e1' e2, from step.eq_left e1_steps,
+        show ∃e', e ⟶ e', from exists.intro (exp.eq e1' e2) this
+      )
+    ),
+    show is_value e ∨ ∃e', e ⟶ e', from or.inr e_steps
+  )
+
+lemma values_not_step {e: exp} (e_is_value: is_value e): ¬ ∃e', e ⟶ e' :=
+  classical.by_contradiction (
+    assume : ¬ ¬ ∃e', e ⟶ e',
+    have e_steps: ∃e', e ⟶ e', from of_not_not this,
+    exists.elim e_steps (
+      assume e': exp,
+      assume e_steps_to_e': e ⟶ e',
+      step_cases e_steps_to_e'
+      ( -- add_case
+        assume n1 n2: ℕ,
+        assume e_is_add: e = exp.add (exp.num n1) (exp.num n2),
+        assume _,
+        have  ¬ is_value (exp.add (exp.num n1) (exp.num n2)), from add_is_not_value,
+        have e_is_not_value: ¬ is_value e, by { rw [←e_is_add] at this, assumption },
+        show false, from absurd e_is_value e_is_not_value
+      )
+      ( -- add_right_case
+        assume e1 e2 e2': exp,
+        assume _ _,
+        assume e_is_add: e = exp.add e1 e2,
+        assume _,
+        have  ¬ is_value (exp.add e1 e2), from add_is_not_value,
+        have e_is_not_value: ¬ is_value e, by { rw [←e_is_add] at this, assumption },
+        show false, from absurd e_is_value e_is_not_value
+      )
+      ( -- add_left_case
+        assume e1 e1' e2: exp,
+        assume _,
+        assume e_is_add: e = exp.add e1 e2,
+        assume _,
+        have  ¬ is_value (exp.add e1 e2), from add_is_not_value,
+        have e_is_not_value: ¬ is_value e, by { rw [←e_is_add] at this, assumption },
+        show false, from absurd e_is_value e_is_not_value
+      )
+      ( -- ite_true_case
+        assume e2 e3: exp,
+        assume e_is_ite: e = exp.ite (exp.bool true) e2 e3,
+        assume _,
+        have  ¬ is_value (exp.ite (exp.bool true) e2 e3), from ite_is_not_value,
+        have e_is_not_value: ¬ is_value e, by { rw [←e_is_ite] at this, assumption },
+        show false, from absurd e_is_value e_is_not_value
+      )
+      ( -- ite_false_case
+        assume e2 e3: exp,
+        assume e_is_ite: e = exp.ite (exp.bool false) e2 e3,
+        assume _,
+        have  ¬ is_value (exp.ite (exp.bool false) e2 e3), from ite_is_not_value,
+        have e_is_not_value: ¬ is_value e, by { rw [←e_is_ite] at this, assumption },
+        show false, from absurd e_is_value e_is_not_value
+      )
+      ( -- ite_case
+        assume e1 e1' e2 e3: exp,
+        assume _,
+        assume e_is_ite: e = exp.ite e1 e2 e3,
+        assume _,
+        have  ¬ is_value (exp.ite e1 e2 e3), from ite_is_not_value,
+        have e_is_not_value: ¬ is_value e, by { rw [←e_is_ite] at this, assumption },
+        show false, from absurd e_is_value e_is_not_value
+      )
+      ( -- eq_num_case
+        assume n1 n2: ℕ,
+        assume e_is_eq: e = exp.eq (exp.num n1) (exp.num n2),
+        assume _,
+        have  ¬ is_value (exp.eq (exp.num n1) (exp.num n2)), from eq_is_not_value,
+        have e_is_not_value: ¬ is_value e, by { rw [←e_is_eq] at this, assumption },
+        show false, from absurd e_is_value e_is_not_value
+      )
+      ( -- eq_bool_case
+        assume b1 b2: bool,
+        assume e_is_eq: e = exp.eq (exp.bool b1) (exp.bool b2),
+        assume _,
+        have  ¬ is_value (exp.eq (exp.bool b1) (exp.bool b2)), from eq_is_not_value,
+        have e_is_not_value: ¬ is_value e, by { rw [←e_is_eq] at this, assumption },
+        show false, from absurd e_is_value e_is_not_value
+      )
+      ( -- eq_right_case
+        assume e1 e2 e2': exp,
+        assume _ _,
+        assume e_is_eq: e = exp.eq e1 e2,
+        assume _,
+        have  ¬ is_value (exp.eq e1 e2), from eq_is_not_value,
+        have e_is_not_value: ¬ is_value e, by { rw [←e_is_eq] at this, assumption },
+        show false, from absurd e_is_value e_is_not_value
+      )
+      ( -- eq_left_case
+        assume e1 e1' e2: exp,
+        assume _,
+        assume e_is_eq: e = exp.eq e1 e2,
+        assume _,
+        have  ¬ is_value (exp.eq e1 e2), from eq_is_not_value,
+        have e_is_not_value: ¬ is_value e, by { rw [←e_is_eq] at this, assumption },
+        show false, from absurd e_is_value e_is_not_value
       )
     )
+  )
+
+lemma add_step_cases {p: Prop} {e1 e2 e': exp} (add_steps: exp.add e1 e2 ⟶ e')
+    (add_case: ∀ (n1 n2: ℕ), e1 = exp.num n1 → e2 = exp.num n2 → e' = exp.num (n1+n2) → p)
+    (add_right_case: ∀e2': exp, is_value e1 → (e2 ⟶ e2') → e' = exp.add e1 e2' → p)
+    (add_left_case: ∀e1': exp, (e1 ⟶ e1') → e' = exp.add e1' e2 → p): p :=
+  step_cases add_steps
+  ( -- add_case
+    assume n1 n2: ℕ,
+    assume add_is_add: exp.add e1 e2 = exp.add (exp.num n1) (exp.num n2),
+    assume e'_is_num: e' = exp.num (n1 + n2),
+    have e1_is_num_n1: e1 = exp.num n1, from and.elim_left (exp.add.inj add_is_add),
+    have e2_is_num_n2: e2 = exp.num n2, from and.elim_right (exp.add.inj add_is_add),
+    show p, from add_case n1 n2 e1_is_num_n1 e2_is_num_n2 e'_is_num
+  )
+  ( -- add_right_case
+    assume e1_ e2_ e2': exp,
+    assume e1__is_value: is_value e1_,
+    assume e2__steps: e2_ ⟶ e2',
+    assume add_is_add: exp.add e1 e2 = exp.add e1_ e2_,
+    assume e'_is_add_: e' = exp.add e1_ e2',
+    have e1_is_e1_: e1 = e1_, from and.elim_left (exp.add.inj add_is_add),
+    have e2_is_e2_: e2 = e2_, from and.elim_right (exp.add.inj add_is_add),
+    have e1_is_value: is_value e1, by { rw[←e1_is_e1_] at e1__is_value, assumption },
+    have e2_steps: e2 ⟶ e2', by { rw[←e2_is_e2_] at e2__steps, assumption },
+    have e'_is_add: e' = exp.add e1 e2', by { rw[←e1_is_e1_] at e'_is_add_, assumption },
+    show p, from add_right_case e2' e1_is_value e2_steps e'_is_add
+  )
+  ( -- add_left_case
+    assume e1_ e1' e2_: exp,
+    assume e1__steps: e1_ ⟶ e1',
+    assume add_is_add: exp.add e1 e2 = exp.add e1_ e2_,
+    assume e'_is_add_: e' = exp.add e1' e2_,
+    have e1_is_e1_: e1 = e1_, from and.elim_left (exp.add.inj add_is_add),
+    have e2_is_e2_: e2 = e2_, from and.elim_right (exp.add.inj add_is_add),
+    have e1_steps: e1 ⟶ e1', by { rw[←e1_is_e1_] at e1__steps, assumption },
+    have e'_is_add: e' = exp.add e1' e2, by { rw[←e2_is_e2_] at e'_is_add_, assumption },
+    show p, from add_left_case e1' e1_steps e'_is_add
+  )
+  ( -- ite_true_case
+    assume e2_ e3_: exp,
+    assume add_is_ite: exp.add e1 e2 = exp.ite (exp.bool true) e2_ e3_,
+    assume _,
+    show p, from exp.no_confusion add_is_ite
+  )
+  ( -- ite_false_case
+    assume e2_ e3_: exp,
+    assume add_is_ite: exp.add e1 e2 = exp.ite (exp.bool false) e2_ e3_,
+    assume _,
+    show p, from exp.no_confusion add_is_ite
+  )
+  ( -- ite_case
+    assume e1_ _ e2_ e3_: exp,
+    assume _,
+    assume add_is_ite: exp.add e1 e2 = exp.ite e1_ e2_ e3_,
+    assume _,
+    show p, from exp.no_confusion add_is_ite
+  )
+  ( -- eq_num_case
+    assume n1 n2: ℕ,
+    assume add_is_eq: exp.add e1 e2 = exp.eq (exp.num n1) (exp.num n2),
+    assume _,
+    show p, from exp.no_confusion add_is_eq
+  )
+  ( -- eq_bool_case
+    assume b1 b2: bool,
+    assume add_is_eq: exp.add e1 e2 = exp.eq (exp.bool b1) (exp.bool b2),
+    assume _,
+    show p, from exp.no_confusion add_is_eq
+  )
+  ( -- eq_right_case
+    assume e1_ e2_ _: exp,
+    assume _ _,
+    assume add_is_eq: exp.add e1 e2 = exp.eq e1_ e2_,
+    assume _,
+    show p, from exp.no_confusion add_is_eq
+  )
+  ( -- eq_left_case
+    assume e1_ _ e2_: exp,
+    assume _,
+    assume add_is_eq: exp.add e1 e2 = exp.eq e1_ e2_,
+    assume _,
+    show p, from exp.no_confusion add_is_eq
+  )
+
+lemma ite_step_cases {p: Prop} {e1 e2 e3 e': exp} (ite_steps: exp.ite e1 e2 e3 ⟶ e')
+    (ite_true_case: e1 = exp.bool true → e' = e2 → p)
+    (ite_false_case: e1 = exp.bool false → e' = e3 → p)
+    (ite_case: ∀e1': exp, (e1 ⟶ e1') → e' = exp.ite e1' e2 e3 → p): p :=
+  step_cases ite_steps
+  ( -- add_case
+    assume n1 n2: ℕ,
+    assume ite_is_add: exp.ite e1 e2 e3 = exp.add (exp.num n1) (exp.num n2),
+    assume _,
+    show p, from exp.no_confusion ite_is_add
+  )
+  ( -- add_right_case
+    assume e1_ e2_ _: exp,
+    assume _ _,
+    assume ite_is_add: exp.ite e1 e2 e3 = exp.add e1_ e2_,
+    assume _,
+    show p, from exp.no_confusion ite_is_add
+  )
+  ( -- add_left_case
+    assume e1_ _ e2_: exp,
+    assume _,
+    assume ite_is_add: exp.ite e1 e2 e3 = exp.add e1_ e2_,
+    assume _,
+    show p, from exp.no_confusion ite_is_add
+  )
+  ( -- ite_true_case
+    assume e2_ e3_: exp,
+    assume ite_is_ite: exp.ite e1 e2 e3 = exp.ite (exp.bool true) e2_ e3_,
+    assume e'_is_e2_: e' = e2_,
+    have e1_is_true: e1 = exp.bool true, from and.elim_left (exp.ite.inj ite_is_ite),
+    have e2_is_e2_: e2 = e2_, from and.elim_left (and.elim_right (exp.ite.inj ite_is_ite)),
+    have e'_is_e2: e' = e2, by { rw[←e2_is_e2_] at e'_is_e2_, assumption },
+    show p, from ite_true_case e1_is_true e'_is_e2
+  )
+  ( -- ite_false_case
+    assume e2_ e3_: exp,
+    assume ite_is_ite: exp.ite e1 e2 e3 = exp.ite (exp.bool false) e2_ e3_,
+    assume e'_is_e3_: e' = e3_,
+    have e1_is_false: e1 = exp.bool false, from and.elim_left (exp.ite.inj ite_is_ite),
+    have e3_is_e3_: e3 = e3_, from and.elim_right (and.elim_right (exp.ite.inj ite_is_ite)),
+    have e'_is_e3: e' = e3, by { rw[←e3_is_e3_] at e'_is_e3_, assumption },
+    show p, from ite_false_case e1_is_false e'_is_e3
+  )
+  ( -- ite_case
+    assume e1_ e1' e2_ e3_: exp,
+    assume e1__steps: e1_ ⟶ e1',
+    assume ite_is_ite: exp.ite e1 e2 e3 = exp.ite e1_ e2_ e3_,
+    assume e'_is_ite_: e' = exp.ite e1' e2_ e3_,
+    have e1_is_e1_: e1 = e1_, from and.elim_left (exp.ite.inj ite_is_ite),
+    have e2_is_e2_: e2 = e2_, from and.elim_left (and.elim_right (exp.ite.inj ite_is_ite)),
+    have e3_is_e3_: e3 = e3_, from and.elim_right (and.elim_right (exp.ite.inj ite_is_ite)),
+    have e1_steps: e1 ⟶ e1', by { rw[←e1_is_e1_] at e1__steps, assumption },
+    have e'_is_ite: e' = exp.ite e1' e2 e3, by { rw[←e2_is_e2_, ←e3_is_e3_] at e'_is_ite_, assumption },
+    show p, from ite_case e1' e1_steps e'_is_ite
+  )
+  ( -- eq_num_case
+    assume n1 n2: ℕ,
+    assume ite_is_eq: exp.ite e1 e2 e3 = exp.eq (exp.num n1) (exp.num n2),
+    assume _,
+    show p, from exp.no_confusion ite_is_eq
+  )
+  ( -- eq_bool_case
+    assume b1 b2: bool,
+    assume ite_is_eq: exp.ite e1 e2 e3 = exp.eq (exp.bool b1) (exp.bool b2),
+    assume _,
+    show p, from exp.no_confusion ite_is_eq
+  )
+  ( -- eq_right_case
+    assume e1_ e2_ _: exp,
+    assume _ _,
+    assume ite_is_eq: exp.ite e1 e2 e3 = exp.eq e1_ e2_,
+    assume _,
+    show p, from exp.no_confusion ite_is_eq
+  )
+  ( -- eq_left_case
+    assume e1_ _ e2_: exp,
+    assume _,
+    assume ite_is_eq: exp.ite e1 e2 e3 = exp.eq e1_ e2_,
+    assume _,
+    show p, from exp.no_confusion ite_is_eq
+  )
+
+lemma eq_step_cases {p: Prop} {e1 e2 e': exp} (eq_steps: exp.eq e1 e2 ⟶ e')
+    (eq_num_case: ∀ (n1 n2: ℕ), e1 = exp.num n1 → e2 = exp.num n2 → e' = exp.bool (n1 = n2) → p)
+    (eq_bool_case: ∀ (b1 b2: bool), e1 = exp.bool b1 → e2 = exp.bool b2 → e' = exp.bool (b1 = b2) → p)
+    (eq_right_case: ∀e2': exp, is_value e1 → (e2 ⟶ e2') → e' = exp.eq e1 e2' → p)
+    (eq_left_case: ∀e1': exp, (e1 ⟶ e1') → e' = exp.eq e1' e2 → p): p :=
+  step_cases eq_steps
+  ( -- add_case
+    assume n1 n2: ℕ,
+    assume eq_is_add: exp.eq e1 e2 = exp.add (exp.num n1) (exp.num n2),
+    assume _,
+    show p, from exp.no_confusion eq_is_add
+  )
+  ( -- add_right_case
+    assume e1_ e2_ _: exp,
+    assume _ _,
+    assume eq_is_add: exp.eq e1 e2 = exp.add e1_ e2_,
+    assume _,
+    show p, from exp.no_confusion eq_is_add
+  )
+  ( -- add_left_case
+    assume e1_ _ e2_: exp,
+    assume _,
+    assume eq_is_add: exp.eq e1 e2 = exp.add e1_ e2_,
+    assume _,
+    show p, from exp.no_confusion eq_is_add
+  )
+  ( -- ite_true_case
+    assume e2_ e3_: exp,
+    assume eq_is_ite: exp.eq e1 e2 = exp.ite (exp.bool true) e2_ e3_,
+    assume _,
+    show p, from exp.no_confusion eq_is_ite
+  )
+  ( -- ite_false_case
+    assume e2_ e3_: exp,
+    assume eq_is_ite: exp.eq e1 e2 = exp.ite (exp.bool false) e2_ e3_,
+    assume _,
+    show p, from exp.no_confusion eq_is_ite
+  )
+  ( -- ite_case
+    assume e1_ _ e2_ e3_: exp,
+    assume _,
+    assume eq_is_ite: exp.eq e1 e2 = exp.ite e1_ e2_ e3_,
+    assume _,
+    show p, from exp.no_confusion eq_is_ite
+  )
+  ( -- eq_num_case
+    assume n1 n2: ℕ,
+    assume eq_is_eq: exp.eq e1 e2 = exp.eq (exp.num n1) (exp.num n2),
+    assume e'_is_num: e' = exp.bool (n1 = n2),
+    have e1_is_num_n1: e1 = exp.num n1, from and.elim_left (exp.eq.inj eq_is_eq),
+    have e2_is_num_n2: e2 = exp.num n2, from and.elim_right (exp.eq.inj eq_is_eq),
+    show p, from eq_num_case n1 n2 e1_is_num_n1 e2_is_num_n2 e'_is_num
+  )
+  ( -- eq_bool_case
+    assume b1 b2: bool,
+    assume eq_is_eq: exp.eq e1 e2 = exp.eq (exp.bool b1) (exp.bool b2),
+    assume e'_is_num: e' = exp.bool (b1 = b2),
+    have e1_is_num_n1: e1 = exp.bool b1, from and.elim_left (exp.eq.inj eq_is_eq),
+    have e2_is_num_n2: e2 = exp.bool b2, from and.elim_right (exp.eq.inj eq_is_eq),
+    show p, from eq_bool_case b1 b2 e1_is_num_n1 e2_is_num_n2 e'_is_num
+  )
+  ( -- eq_right_case
+    assume e1_ e2_ e2': exp,
+    assume e1__is_value: is_value e1_,
+    assume e2__steps: e2_ ⟶ e2',
+    assume e_is_eq: exp.eq e1 e2 = exp.eq e1_ e2_,
+    assume e'_is_eq_: e' = exp.eq e1_ e2',
+    have e1_is_e1_: e1 = e1_, from and.elim_left (exp.eq.inj e_is_eq),
+    have e2_is_e2_: e2 = e2_, from and.elim_right (exp.eq.inj e_is_eq),
+    have e1_is_value: is_value e1, by { rw[←e1_is_e1_] at e1__is_value, assumption },
+    have e2_steps: e2 ⟶ e2', by { rw[←e2_is_e2_] at e2__steps, assumption },
+    have e'_is_eq: e' = exp.eq e1 e2', by { rw[←e1_is_e1_] at e'_is_eq_, assumption },
+    show p, from eq_right_case e2' e1_is_value e2_steps e'_is_eq
+  )
+  ( -- eq_left_case
+    assume e1_ e1' e2_: exp,
+    assume e1__steps: e1_ ⟶ e1',
+    assume e_is_eq: exp.eq e1 e2 = exp.eq e1_ e2_,
+    assume e'_is_eq_: e' = exp.eq e1' e2_,
+    have e1_is_e1_: e1 = e1_, from and.elim_left (exp.eq.inj e_is_eq),
+    have e2_is_e2_: e2 = e2_, from and.elim_right (exp.eq.inj e_is_eq),
+    have e1_steps: e1 ⟶ e1', by { rw[←e1_is_e1_] at e1__steps, assumption },
+    have e'_is_eq: e' = exp.eq e1' e2, by { rw[←e2_is_e2_] at e'_is_eq_, assumption },
+    show p, from eq_left_case e1' e1_steps e'_is_eq
+  )
+
+theorem preservation(e: exp) (t: typ) (e_typed_t: e ::: t): (∀e': exp, e ⟶ e' → (e' ::: t)) :=
+  typed.rec_on e_typed_t
+  ( -- num
+    assume n: ℕ,
+    let e := exp.num n in
+    let t := typ.num in
+    assume e': exp,
+    assume e_steps: e ⟶ e',
+    have e_can_step: (∃e', e ⟶ e'), from exists.intro e' e_steps,
+    have e_is_value: is_value e, from is_value.num,
+    show e' ::: t, from absurd e_can_step (values_not_step e_is_value)
+  )
+  ( -- bool
+    assume b: bool,
+    let e := exp.bool b in
+    let t := typ.bool in
+    assume e': exp,
+    assume e_steps: e ⟶ e',
+    have e_can_step: (∃e', e ⟶ e'), from exists.intro e' e_steps,
+    have e_is_value: is_value e, from is_value.bool,
+    show e' ::: t, from absurd e_can_step (values_not_step e_is_value)
+  )
+  ( -- add
+    assume e1 e2: exp,
+    let e := exp.add e1 e2 in
+    let t := typ.num in
+    assume e1_typed_num : e1 ::: typ.num,
+    assume e2_typed_num : e2 ::: typ.num,
+    assume e1ih: (∀e1': exp, e1 ⟶ e1' → (e1' ::: typ.num)),
+    assume e2ih: (∀e2': exp, e2 ⟶ e2' → (e2' ::: typ.num)),
+    assume e': exp,
+    assume e_steps: e ⟶ e',
+    have e_is_add: e = exp.add e1 e2, from rfl,
+    have exp.add e1 e2 ⟶ e', by { rw[e_is_add] at e_steps, assumption },
+    add_step_cases this
+    ( -- add_case
+      assume n1 n2: ℕ,
+      assume e1_is_num_n1: e1 = exp.num n1,
+      assume e2_is_num_n2: e2 = exp.num n2,
+      assume e'_is_num: e' = exp.num (n1 + n2),
+      have exp.num (n1 + n2) ::: typ.num, from typed.num,
+      show e' ::: t, by { rw[←e'_is_num] at this, assumption }
+    )
+    ( -- add_right_case
+      assume e2': exp,
+      assume e1_is_value: is_value e1,
+      assume e2_steps: e2 ⟶ e2',
+      assume e'_is_add: e' = exp.add e1 e2',
+      have e2'_typed_num: e2' ::: typ.num, from e2ih e2' e2_steps,
+      have exp.add e1 e2' ::: typ.num, from typed.add e1_typed_num e2'_typed_num,
+      show e' ::: t, by { rw[←e'_is_add] at this, assumption }
+    )
+    ( -- add_left_case
+      assume e1': exp,
+      assume e1_steps: e1 ⟶ e1',
+      assume e'_is_add: e' = exp.add e1' e2,
+      have e1'_typed_num: e1' ::: typ.num, from e1ih e1' e1_steps,
+      have exp.add e1' e2 ::: typ.num, from typed.add e1'_typed_num e2_typed_num,
+      show e' ::: t, by { rw[←e'_is_add] at this, assumption }
+    )
+  )
+  ( -- ite
+    assume e1 e2 e3: exp,
+    let e := exp.ite e1 e2 e3 in
+    assume t: typ,
+    assume e1_is_bool: e1 ::: typ.bool,
+    assume e2_typed_t: e2 ::: t,
+    assume e3_typed_t: e3 ::: t,
+    assume e1ih: (∀e1': exp, e1 ⟶ e1' → (e1' ::: typ.bool)),
+    assume e2ih: (∀e2': exp, e2 ⟶ e2' → (e2' ::: t)),
+    assume e3ih: (∀e3': exp, e3 ⟶ e3' → (e3' ::: t)),
+    assume e': exp,
+    assume e_steps: e ⟶ e',
+    have e_is_ite: e = exp.ite e1 e2 e3, from rfl,
+    have exp.ite e1 e2 e3 ⟶ e', by { rw[e_is_ite] at e_steps, assumption },
+    ite_step_cases this
+    ( -- ite_true_case
+      assume e1_is_true: e1 = exp.bool true,
+      assume e'_is_e2: e' = e2,
+      show e' ::: t, by { rw[←e'_is_e2] at e2_typed_t, assumption } 
+    )
+    ( -- ite_false_case
+      assume e1_is_false: e1 = exp.bool false,
+      assume e'_is_e3: e' = e3,
+      show e' ::: t, by { rw[←e'_is_e3] at e3_typed_t, assumption } 
+    )
+    ( -- ite_case
+      assume e1': exp,
+      assume e1_steps: e1 ⟶ e1',
+      assume e'_is_ite: e' = exp.ite e1' e2 e3,
+      have e1'_typed_bool: e1' ::: typ.bool, from e1ih e1' e1_steps,
+      have exp.ite e1' e2 e3 ::: t, from typed.ite e1'_typed_bool e2_typed_t e3_typed_t,
+      show e' ::: t, by { rw[←e'_is_ite] at this, assumption }
+    )
+  )
+  ( -- eq
+    assume e1 e2: exp,
+    assume t1: typ,
+    let e := exp.eq e1 e2 in
+    let t := typ.bool in
+    assume e1_typed_t1 : e1 ::: t1,
+    assume e2_typed_t1 : e2 ::: t1,
+    assume e1ih: (∀e1': exp, e1 ⟶ e1' → (e1' ::: t1)),
+    assume e2ih: (∀e2': exp, e2 ⟶ e2' → (e2' ::: t1)),
+    assume e': exp,
+    assume e_steps: e ⟶ e',
+    have e_is_eq: e = exp.eq e1 e2, from rfl,
+    have exp.eq e1 e2 ⟶ e', by { rw[e_is_eq] at e_steps, assumption },
+    eq_step_cases this
+    ( -- eq_num_case
+      assume n1 n2: ℕ,
+      assume _ _,
+      assume e'_is_bool: e' = exp.bool (n1 = n2),
+      have exp.bool (n1 = n2) ::: typ.bool, from typed.bool,
+      show e' ::: t, by { rw[←e'_is_bool] at this, assumption }
+    )
+    ( -- eq_bool_case
+      assume b1 b2: bool,
+      assume _ _,
+      assume e'_is_bool: e' = exp.bool (b1 = b2),
+      have exp.bool (b1 = b2) ::: typ.bool, from typed.bool,
+      show e' ::: t, by { rw[←e'_is_bool] at this, assumption }
+    )
+    ( -- eq_right_case
+      assume e2': exp,
+      assume e1_is_value: is_value e1,
+      assume e2_steps: e2 ⟶ e2',
+      assume e'_is_eq: e' = exp.eq e1 e2',
+      have e2'_typed_t1: e2' ::: t1, from e2ih e2' e2_steps,
+      have exp.eq e1 e2' ::: typ.bool, from typed.eq e1_typed_t1 e2'_typed_t1,
+      show e' ::: t, by { rw[←e'_is_eq] at this, assumption }
+    )
+    ( -- eq_left_case
+      assume e1': exp,
+      assume e1_steps: e1 ⟶ e1',
+      assume e'_is_eq: e' = exp.eq e1' e2,
+      have e1'_typed_t1: e1' ::: t1, from e1ih e1' e1_steps,
+      have exp.eq e1' e2 ::: typ.bool, from typed.eq e1'_typed_t1 e2_typed_t1,
+      show e' ::: t, by { rw[←e'_is_eq] at this, assumption }
+    )
+  )
+
+theorem does_not_get_stuck {e e': exp} (e_steps: e ⟶* e'): ∀t: typ, e ::: t → is_value e' ∨ ∃e'', e' ⟶ e'' :=
+  trans_step.rec_on e_steps
+  ( -- e
+    assume e: exp,
+    assume t: typ,
+    assume e_typed_t: e ::: t,
+    show is_value e ∨ ∃e', e ⟶ e', from progress e t e_typed_t
+  )
+  (
+    assume e e' e'': exp,
+    assume e_step: e ⟶ e',
+    assume e'_steps: e' ⟶* e'',
+    assume ih: ∀t': typ, e' ::: t' → is_value e'' ∨ ∃e''', e'' ⟶ e''',
+    assume t: typ,
+    assume e_typed_t: e ::: t,
+    have e'_typed_t: e' ::: t, from preservation e t e_typed_t e' e_step,
+    show is_value e'' ∨ ∃e''', e'' ⟶ e''', from ih t e'_typed_t
+  )
 
 end arith
